prove Sequent.allSeqt_subseteq_FL_complete, still needs allNegLoads

Pdl/TableauGame.lean
@@ -447,11 +447,50 @@ is not allowed.
 
 -/
 
-lemma move_inside_FL (mov : move p next) : next.2.1.subseteq_FL p.2.1 := by
+lemma move_inside_FL {p next} (mov : move p next) : next.2.1.subseteq_FL p.2.1 := by
   cases mov
   case prPdl r => apply PdlRule.stays_in_FL r
   case buEnd ltX _ _ _ _ Y_in => simp; apply LocalTableau.stays_in_FL ltX _ Y_in
   case prLocTab => simp
+
+/-- Given `~⌈α₁⌉…⌈αₙ⌉φ`, return the list of `~⌊α₁⌋…⌊αₖ⌋⌈αₖ₊₁⌉…⌈αₙ⌉φ` for all k. -/
+def Formula.allNegLoads : Formula → List NegLoadFormula
+| ~φ => match boxesOf φ with
+  | ([],_) => []
+  | (α::αs,ψ) => match h : splitLast (α::αs) with
+    | none => by exfalso; grind [splitLast_cons_eq_some]
+    | some (βs, β) => (~'⌊⌊βs⌋⌋⌊β⌋ψ) :: do
+        let k ← List.range' 0 (αs.length-1)
+        let (front,back) := αs.splitAt k -- not getting a proof here?!
+        match h' : splitLast front with
+          | none => by exfalso; sorry
+          | some (γs, γ) => return (~'⌊⌊γs⌋⌋⌊γ⌋⌈⌈back⌉⌉⌈β⌉ψ) -- CHECK THIS ?!?
+| _ => []
+
+lemma Formula.allNegLoads_spec {nχ φ} :
+    nχ ∈ φ.allNegLoads → negUnload nχ = φ := by
+  cases φ <;> simp [allNegLoads]
+  case neg χ =>
+  cases χ <;> simp_all [boxesOf]
+  case box α φ =>
+    rcases nχ with ⟨χ⟩
+    split
+    next h =>
+      intro nχ_in
+      absurd h
+      simp [splitLast_cons_eq_some]
+    next γs γ h =>
+      -- better rewrite `Formula.allNegLoads` first?
+      sorry
+
+lemma Formula.allNegLoads_complete {nχ φ} :
+    negUnload nχ = φ → nχ ∈ φ.allNegLoads := by
+  rcases nχ with ⟨χ⟩
+  simp [negUnload]
+  intro def_φ
+  subst def_φ
+  simp [allNegLoads]
+  sorry
 
 /-- A list of sequents that are all FL-subsequents of the given sequent.
 The list defined here is not complete because there are infinitely many such other sequents.
@@ -466,19 +505,47 @@ def Sequent.all_subseteq_FL (Y : Sequent) : List { X : Sequent // Sequent.subset
   let XOL ← (FLL (Y.L ++ Y.O.L)).sublists.attach
   let XR  ← (FLL (Y.R ++ Y.O.R)).sublists.attach
   let XOR ← (FLL (Y.R ++ Y.O.R)).sublists.attach
-  -- TODO: We need to generate all possible `XO : Olf` from `XOL` and `XOR` here.
-  let X : Sequent := ⟨XL.1, XR.1, none⟩
+  -- Now we still need to generate all possible `XO : Olf` from `XOL` and `XOR`.
+  let OLs : List Olf:= XOL.1.flatMap (fun φ => φ.allNegLoads.map (some ∘ Sum.inl))
+  let ORs : List Olf:= XOR.1.flatMap (fun φ => φ.allNegLoads.map (some ∘ Sum.inr))
+  let XO ← ((none : Olf) :: OLs ++ ORs).attach
+  let X : Sequent := ⟨XL.1, XR.1, XO.1⟩
   have h : X.subseteq_FL Y := by
     unfold X
     rcases Y with ⟨L',R',O'⟩
-    refine ⟨?_, ?_, ?_⟩ <;> simp
+    refine ⟨?_, ?_, ?_, ?_⟩ <;> simp
     · have := XL.2
       simp at this
       exact List.Sublist.subset this
+    · simp only [Olf.L]
+      rcases XO with ⟨none|⟨(nχ|_)⟩, XO_in⟩ <;> try simp_all
+      simp only [List.cons_append, List.mem_cons, reduceCtorEq, List.mem_append, List.mem_flatMap,
+        List.mem_map, Function.comp_apply, Option.some.injEq, Sum.inl.injEq, exists_eq_right,
+        and_false, exists_false, or_false, false_or, OLs, ORs] at XO_in
+      rcases XO_in with ⟨φ, φ_in, nχ_in⟩
+      have := Formula.allNegLoads_spec nχ_in
+      simp only [negUnload] at this
+      rw [this]
+      suffices φ ∈ (FLL (L' ++ O'.L)) by aesop
+      have := XOL.2
+      simp only [L_eq, O_eq, List.mem_sublists] at this
+      exact List.Sublist.mem φ_in this
     · have := XR.2
-      simp at this
+      simp only [R_eq, O_eq, List.mem_sublists] at this
       exact List.Sublist.subset this
-    -- · sorry -- TODO for O later
+    · simp only [Olf.R]
+      rcases XO with ⟨none|⟨(nχ|_)⟩, XO_in⟩ <;> try simp_all
+      simp only [List.cons_append, List.mem_cons, reduceCtorEq, List.mem_append, List.mem_flatMap,
+        List.mem_map, Function.comp_apply, Option.some.injEq, and_false, exists_false,
+        Sum.inr.injEq, exists_eq_right, false_or, OLs, ORs] at XO_in
+      rcases XO_in with ⟨φ, φ_in, nχ_in⟩
+      have := Formula.allNegLoads_spec nχ_in
+      simp only [negUnload] at this
+      rw [this]
+      suffices φ ∈ (FLL (R' ++ O'.R)) by aesop
+      have := XOR.2
+      simp only [R_eq, O_eq, List.mem_sublists] at this
+      exact List.Sublist.mem φ_in this
   return ⟨X, h⟩
 
 /-! NOTE
@@ -590,15 +657,76 @@ lemma Sequent.allSeqt_subseteq_FL_spec (X : Sequent) :
   rcases Ys_in with ⟨Z, ⟨Z_sub_X, Z_in_all⟩, Z_equiv_Y⟩
   exact Sequent.subseteq_FL_of_setEq_left Z_equiv_Y Z_sub_X
 
+/-- Small helper function. Mathlib this? -/
+lemma exists_mem_sublists_toFinsetEq_of_Subset [DecidableEq α] {A B : List α} :
+    A ⊆ B → ∃ C ∈ B.sublists, C.toFinset = A.toFinset := by
+  intro A_sub_B
+  use (List.filter (fun x => decide (x ∈ A)) B)
+  simp only [List.mem_sublists, List.filter_sublist, List.toFinset_filter, decide_eq_true_eq,
+    true_and]
+  aesop
+
 lemma Sequent.allSeqt_subseteq_FL_complete (X : Sequent) :
     ∀ Y, Y.subseteq_FL X → ⟦Y⟧ ∈ X.allSeqt_subseteq_FL := by
   intro Y Y_in
-  simp [Sequent.allSeqt_subseteq_FL, instSetoidSequent]
+  simp only [instSetoidSequent, allSeqt_subseteq_FL, List.map_subtype, List.mem_toFinset,
+    List.mem_map, List.mem_unattach, Quotient.eq]
   -- Here the above NOTE matters.
   -- We need to work around that there is no `Sequent.all_subseteq_FL_complete`.
-  -- use Y -- this might not work because `Y` might not be in `all_subseteq_FL`.
-  -- How to find a sequent that is an element of `all_subseteq_FL` ???
-  sorry
+  -- `use Y` would not work because `Y` might not be in `all_subseteq_FL`.
+  -- Instead, we find something that is `setEqTo Y` but also an element of `all_subseteq_FL`.
+  unfold subseteq_FL at Y_in
+  rcases Y_in with ⟨Lh, OLh, Rh, ORh⟩
+  -- Now use the lemma that for any subset of a list gives us a sublist, four times.
+  rcases exists_mem_sublists_toFinsetEq_of_Subset Lh  with ⟨L' , L'_in , L'_same ⟩
+  rcases exists_mem_sublists_toFinsetEq_of_Subset OLh with ⟨OL', OL'_in, OL'_same⟩
+  rcases exists_mem_sublists_toFinsetEq_of_Subset Rh  with ⟨R' , R'_in , R'_same ⟩
+  rcases exists_mem_sublists_toFinsetEq_of_Subset ORh with ⟨OR', OR'_in, OR'_same⟩
+  -- Now we need to reconstruct (a subOption of ???) `Y.O` from OL' and R' here ??
+  -- Or could we just use Y.O itself ?!?!
+  refine ⟨⟨L', R', Y.O⟩, ⟨?_, ?_⟩ , L'_same, R'_same, rfl⟩
+  · unfold subseteq_FL
+    simp only [L_eq, O_eq, R_eq]
+    simp_all [FLL_append_eq]
+    constructor
+    · exact List.Sublist.subset L'_in
+    · exact List.Sublist.subset R'_in
+  · rcases Y with ⟨YL, YR, YO⟩
+    rcases X with ⟨XL, XR, XO⟩
+    -- now we hope that the above procedure imitates the `all_subseteq_FL` def :-)
+    simp only [all_subseteq_FL, L, R, O]
+    simp only [List.cons_append, List.attach_cons, List.attach_append, List.map_append,
+      List.map_map, List.pure_def, List.bind_eq_flatMap, List.flatMap_cons, List.flatMap_append,
+      List.nil_append, List.mem_flatMap, List.mem_attach, List.mem_cons, Subtype.mk.injEq,
+      List.mem_append, List.mem_map, Function.comp_apply, true_and, Subtype.exists,
+      List.not_mem_nil, or_false, exists_prop, exists_eq_right, List.mem_sublists]
+    refine ⟨L', List.mem_sublists.mp L'_in, ?_⟩
+    refine ⟨OL', List.mem_sublists.mp OL'_in, ?_⟩
+    refine ⟨R', List.mem_sublists.mp R'_in, ?_⟩
+    refine ⟨OR', List.mem_sublists.mp OR'_in, ?_⟩
+    rcases YO with none|⟨nχ|nχ⟩
+    · left; rfl
+    · right; left
+      have nχ_in : negUnload nχ ∈ OL' := by
+        simp only [O_eq, Olf.L_inl, List.toFinset_cons, List.toFinset_nil,
+          insert_empty_eq, negUnload] at *
+        rw [← List.mem_toFinset, OL'_same]
+        simp
+      refine ⟨some (Sum.inl nχ), ?_, ⟨?_, rfl⟩⟩
+      · right; left
+        exact ⟨negUnload nχ, nχ_in, ⟨nχ, Formula.allNegLoads_complete rfl, rfl⟩⟩
+      · exact ⟨negUnload nχ, nχ_in, ⟨nχ, Formula.allNegLoads_complete rfl, rfl⟩⟩
+    · right; right
+      have nχ_in : negUnload nχ ∈ OR' := by
+        simp only [L_eq, O_eq, List.mem_sublists, R_eq, Olf.L_inr, List.toFinset_nil,
+          List.toFinset_eq_empty_iff, Olf.R_inr, List.toFinset_cons, insert_empty_eq,
+          List.nil_subset, List.cons_subset, and_true, negUnload] at *
+        rw [← List.mem_toFinset, OR'_same]
+        simp
+      refine ⟨some (Sum.inr nχ), ?_, ⟨?_, rfl⟩⟩
+      · right; right
+        exact ⟨negUnload nχ, nχ_in, ⟨nχ, Formula.allNegLoads_complete rfl, rfl⟩⟩
+      · exact ⟨negUnload nχ, nχ_in, ⟨nχ, Formula.allNegLoads_complete rfl, rfl⟩⟩
 
 lemma Sequent.allSeqt_subseteq_FL_congr (X Y : Sequent) (h : X ≈ Y) :
     Sequent.allSeqt_subseteq_FL X = Sequent.allSeqt_subseteq_FL Y := by
@@ -625,11 +753,18 @@ def Seqt.all_subseteq_FL (Xs : Seqt) : Finset Seqt  :=
 
 lemma Seqt.all_subseteq_FL_spec {Ys : Seqt} (Ys_in : Ys ∈ Xs.all_subseteq_FL) :
     Ys.subseteq_FL Xs := by
-  sorry
+  rcases Ys with ⟨Y⟩
+  rcases Xs with ⟨x⟩
+  unfold Seqt.all_subseteq_FL at Ys_in
+  unfold Seqt.subseteq_FL
+  simp [instSetoidSequent] at *
+  exact Sequent.allSeqt_subseteq_FL_spec x Y Ys_in
 
 lemma Seqt.all_subseteq_FL_complete {Ys : Seqt} (Ys_in : Ys.subseteq_FL Xs) :
     Ys ∈ Xs.all_subseteq_FL := by
-  sorry
+  rcases Ys with ⟨Y⟩
+  rcases Xs with ⟨X⟩
+  exact Sequent.allSeqt_subseteq_FL_complete X Y Ys_in
 
 def Seqt.all_subseteq_FL_attached (Xs : Seqt) : Finset { Ys :Seqt // Ys.subseteq_FL Xs } :=
   Xs.all_subseteq_FL.attach.map
